src/goose_lang/refinement_adequacy.v
@@ -528,10 +528,11 @@ Proof using Hrpre Hhpre Hcpre.
     iDestruct (oracle_agree with "Hor_auth Horacle_frag") as %Heq2'.
 
     iInv "Hpre_inv" as ">H" "Hclo".
+    iApply physical_step2_intro. iIntros "Hcl".
     iMod (physical_step_use_pre_borrowN with "[$]") as "_".
     iPoseProof (@Hwp_crash $! _ _ with "HΦc") as "H".
     iApply physical_step_intro.
-    iNext. iIntros "[Hbor1 Hbor2]".
+    iNext. iIntros "[Hbor1 Hbor2]". iMod "Hcl". iModIntro.
     iMod ("Hclo" with "[$]") as "_".
     iMod (na_heap.na_heap_reinit _ tls σ_post_crash.(heap)) as (name_na_heap) "Hh".
     iDestruct "Hg" as "(Hffig&Hg)".
