src/program_logic/staged_invariant_use_idle.v
@@ -169,9 +169,11 @@ Proof using later_tokG0.
     replace (⊤ ∖ D ∖ E2) with (⊤ ∖ (E2 ∪ D)) by set_solver.
     iDestruct ("Hwp" with "[$] [$] [$]") as "Hwp".
     iModIntro. iSplit; [by iLeft in "Hwp"|iRight in "Hwp"].
-    iIntros (e2 ????). iMod "Hcl" as "_".
-    iApply (physical_step_wand with "(Hwp [//])").
-    iIntros "($&Hg&H&Hefs&HNC) [[Htok _]_]".
+    iIntros (e2 ????).
+    iApply (physical_step2_step_update with "[Hcl]").
+    { iMod "Hcl". iIntros "!> /= [Htok _]". iExact "Htok". }
+    iApply (physical_step2_wand_later with "(Hwp [//])"); [done..|].
+    iIntros "!> ($&Hg&H&Hefs&HNC) Htok".
     destruct (to_val e2) eqn:Heq_val.
     {
       iEval (rewrite wpc0_unfold /wpc_pre) in "H".
@@ -364,9 +366,11 @@ Proof using later_tokG0.
   replace (⊤ ∖ D ∖ E2) with (⊤ ∖ (E2 ∪ D)) by set_solver.
   iDestruct ("Hwp" with "[$] [$] [$]") as "Hwp".
   iModIntro. iSplit; [by iLeft in "Hwp"|iRight in "Hwp"].
-  iIntros (e2 ????). iMod "Hcl" as "_".
-  iApply (physical_step_wand with "(Hwp [//])").
-  iIntros "($&Hg&H&Hefs&HNC) [[Htok _] _]".
+  iIntros (e2 ????).
+  iApply (physical_step2_step_update with "[Hcl]").
+  { iMod "Hcl". iIntros "!> /= [Htok _]". iExact "Htok". }
+  iApply (physical_step2_wand_later with "(Hwp [//])"); [done..|].
+  iIntros "!> ($&Hg&H&Hefs&HNC) Htok".
   destruct (to_val e2) eqn:Heq_val.
   {
     iEval (rewrite wpc0_unfold /wpc_pre) in "H".
