src/program_logic/staged_invariant_use_inuse2.v
@@ -167,10 +167,10 @@ Proof using later_tokG0.
     iDestruct ("Hwp" with "[$] [$] [$]") as "Hwp". iModIntro.
     iSplit; [by iLeft in "Hwp"|iRight in "Hwp"].
     iIntros (e2 ????).
-
-    iMod "Hcl" as "_". simpl.
-    iApply (physical_step_wand with "(Hwp [//])").
-    iIntros "($&Hg&H&Hefs&HNC) [Htok _]".
+    iApply (physical_step2_step_update with "[Hcl]").
+    { iMod "Hcl". iIntros "!> /= [Htok _]". iExact "Htok". }
+    iApply (physical_step2_wand_later with "(Hwp [//])"); [done..|].
+    iIntros "!> ($&Hg&H&Hefs&HNC) Htok".
 
     destruct (to_val e2) eqn:Heq_val.
     {
@@ -360,9 +360,10 @@ Proof using later_tokG0.
   iDestruct ("Hwp" with "[$] [$] [$]") as "Hwp".
   iModIntro. iSplit; [by iLeft in "Hwp"|iRight in "Hwp"].
   iIntros (e2 σ2 g2 efs Hstep).
-  iMod "Hcl" as "_". simpl.
-  iApply (physical_step_wand with "(Hwp [//])").
-  iIntros "($&Hg&H&Hefs&HNC) [Htok _]".
+  iApply (physical_step2_step_update with "[Hcl]").
+  { iMod "Hcl". iIntros "!> /= [Htok _]". iExact "Htok". }
+  iApply (physical_step2_wand_later with "(Hwp [//])"); [done..|].
+  iIntros "!> ($&Hg&H&Hefs&HNC) Htok".
 
   destruct (to_val e2) eqn:Heq_val.
   {
